

Calculation For Hamiltonians

-Hadamard Gate Realization

1. $U_H = a_x X + a_y Y + a_z Z + a_0 I$
2. $a_x = \frac{1}{2} \text{Tr}[X U_H] = \frac{1}{2\sqrt{2}} \text{Tr}\left[\begin{pmatrix} 0 & 1 \\ 1 & 0 \end{pmatrix} \begin{pmatrix} 1 & 1 \\ 1 & -1 \end{pmatrix}\right]$
3. $a_x = \frac{1}{2\sqrt{2}} \text{Tr}\left[\begin{pmatrix} 1 & -1 \\ 1 & 1 \end{pmatrix}\right] = \frac{1}{\sqrt{2}}$
4. $a_y = \frac{1}{2} \text{Tr}[Y U_H] = \frac{i}{2\sqrt{2}} \text{Tr}\left[\begin{pmatrix} 0 & -1 \\ 1 & 0 \end{pmatrix} \begin{pmatrix} 1 & 1 \\ 1 & -1 \end{pmatrix}\right]$
5. $= \frac{i}{2\sqrt{2}} \text{Tr}\left[\begin{pmatrix} -1 & 1 \\ 1 & 1 \end{pmatrix}\right] = 0$
6. $a_z = \frac{1}{2} \text{Tr}[Z U_H] = \frac{1}{2\sqrt{2}} \text{Tr}\left[\begin{pmatrix} 1 & 0 \\ 0 & -1 \end{pmatrix} \begin{pmatrix} 1 & 1 \\ 1 & -1 \end{pmatrix}\right]$
7. $= \frac{1}{2\sqrt{2}} \text{Tr}\left[\begin{pmatrix} 1 & 1 \\ -1 & 1 \end{pmatrix}\right] = \frac{1}{\sqrt{2}}$
8. $a_0 = \frac{1}{2} \text{Tr}[U_H] = \frac{1}{2\sqrt{2}} \text{Tr}\left[\begin{pmatrix} 1 & 1 \\ 1 & -1 \end{pmatrix}\right] = 0$
9. $U_H = \frac{1}{\sqrt{2}} (X + Z)$
10. $U_H = \frac{1}{\sqrt{2}} \left(\begin{bmatrix} 0 & 1 \\ 1 & 0 \end{bmatrix} + \begin{bmatrix} 1 & 0 \\ 0 & -1 \end{bmatrix} \right)$
11. $U_H = \frac{1}{\sqrt{2}} \begin{bmatrix} 1 & 1 \\ 1 & -1 \end{bmatrix}$

Calculations For Hamiltonians

- Hadamard Gate Hamiltonian

$$1. \sigma = \frac{1}{\sqrt{2}} \begin{bmatrix} 1 & 1 \\ 1 & -1 \end{bmatrix}$$

$$2. H_H = -\frac{b}{2} \sigma$$

$$3. H_H = -\frac{b}{2\sqrt{2}} \begin{bmatrix} 1 & 1 \\ 1 & -1 \end{bmatrix}$$

Calculations For Hamiltonian

- Hadamard Gate realization
for 2 qubit system

$$1. U_{H12} \equiv U_H \otimes U_H$$

$$2. = \frac{1}{2} \begin{bmatrix} 1 & 1 \\ 1 & -1 \end{bmatrix} \otimes \begin{bmatrix} 1 & 1 \\ 1 & -1 \end{bmatrix}$$

$$3. = \frac{1}{2} \begin{bmatrix} 1 \begin{bmatrix} 1 & 1 \\ 1 & -1 \end{bmatrix} & 1 \begin{bmatrix} 1 & 1 \\ 1 & -1 \end{bmatrix} \\ 1 \begin{bmatrix} 1 & 1 \\ 1 & -1 \end{bmatrix} & -1 \begin{bmatrix} 1 & 1 \\ 1 & -1 \end{bmatrix} \end{bmatrix}$$

$$4. = \frac{1}{2} \begin{bmatrix} 1 & 1 & 1 & 1 \\ 1 & -1 & 1 & -1 \\ 1 & 1 & -1 & -1 \\ 1 & -1 & -1 & 1 \end{bmatrix}$$

Calculations For Hamiltonians

- Hadamard Gate Hamiltonian
For 2 qubit system

$$1. U_{H_{12}} = \frac{1}{2} \begin{bmatrix} 1 & 1 & 1 & 1 \\ 1 & -1 & 1 & -1 \\ 1 & 1 & -1 & -1 \\ 1 & -1 & -1 & 1 \end{bmatrix}$$

$$2. H_{12} = -\frac{b}{2} U_{H_{12}}$$

$$3. H_{12} = -\frac{b}{4} \begin{bmatrix} 1 & 1 & 1 & 1 \\ 1 & -1 & 1 & -1 \\ 1 & 1 & -1 & -1 \\ 1 & -1 & -1 & 1 \end{bmatrix}$$

Calculations For Hamiltonians

- Z Gate Hamiltonian

$$H_Z = \frac{b}{2} Z$$

- Z Gate Hamiltonian

for 2 qubit system in which second qubit is targeted

$$1. Z_2 = I \otimes Z = \begin{bmatrix} 1 & 0 \\ 0 & 1 \end{bmatrix} \otimes \begin{bmatrix} 1 & 0 \\ 0 & -1 \end{bmatrix}$$

$$2. = \begin{bmatrix} 1 \begin{bmatrix} 1 & 0 \\ 0 & -1 \end{bmatrix} & 0 \begin{bmatrix} 1 & 0 \\ 0 & -1 \end{bmatrix} \\ 0 \begin{bmatrix} 1 & 0 \\ 0 & -1 \end{bmatrix} & 1 \begin{bmatrix} 1 & 0 \\ 0 & -1 \end{bmatrix} \end{bmatrix}$$

$$3. = \begin{bmatrix} 1 & 0 & 0 & 0 \\ 0 & -1 & 0 & 0 \\ 0 & 0 & 1 & 0 \\ 0 & 0 & 0 & -1 \end{bmatrix}$$

$$4. H_{Z_2} = \frac{b}{2} \begin{bmatrix} 1 & 0 & 0 & 0 \\ 0 & -1 & 0 & 0 \\ 0 & 0 & 1 & 0 \\ 0 & 0 & 0 & -1 \end{bmatrix}$$

1. Initial state $|\psi(0)\rangle = |00\rangle$

2. $\rho(0) = |00\rangle\langle 00|$

$$= \begin{bmatrix} 1 \\ 0 \\ 0 \\ 0 \end{bmatrix} \begin{bmatrix} 1 & 0 & 0 & 0 \end{bmatrix} = \begin{bmatrix} 1 & 0 & 0 & 0 \\ 0 & 0 & 0 & 0 \\ 0 & 0 & 0 & 0 \\ 0 & 0 & 0 & 0 \end{bmatrix}$$

3. Unitary Operator $U(t)$

$$U(t) = e^{-iHt/\hbar}$$

Generic Form

4. $\rho(t) = U(t)\rho(0)U^\dagger(t)$

5.
$$= e^{-iHt/\hbar} \begin{bmatrix} 1 & 0 & 0 & 0 \\ 0 & 0 & 0 & 0 \\ 0 & 0 & 0 & 0 \\ 0 & 0 & 0 & 0 \end{bmatrix} e^{iHt/\hbar}$$

6. Form when Hadamard Gate is applied

7. $\rho(t) = U(t)\rho(0)U^\dagger(t)$

8.
$$= e^{-iH_1 t/\hbar} \begin{bmatrix} 1 & 0 & 0 & 0 \\ 0 & 0 & 0 & 0 \\ 0 & 0 & 0 & 0 \\ 0 & 0 & 0 & 0 \end{bmatrix} e^{iH_1 t/\hbar}$$

9.
$$= e^{-iU_H b t/\hbar} \begin{bmatrix} 1 & 0 & 0 & 0 \\ 0 & 0 & 0 & 0 \\ 0 & 0 & 0 & 0 \\ 0 & 0 & 0 & 0 \end{bmatrix} e^{iU_H b t/\hbar}$$

10. + value corresponding
to a π rotation around
 $(\hat{x} + \hat{z})/2$ axis

$$11. \frac{b t}{4\hbar} = \frac{\pi}{4}$$

$$12. t = \frac{4\pi\hbar}{4b} = \frac{\pi\hbar}{b}$$

13. Form when Z Gate is applied

$$14. \rho(t) = U(t) \rho(0) U^\dagger(t)$$

$$15. = e^{-iH_Z t/\hbar} \begin{bmatrix} 1 & 0 & 0 & 0 \\ 0 & 0 & 0 & 0 \\ 0 & 0 & 0 & 0 \\ 0 & 0 & 0 & 0 \end{bmatrix} e^{iH_Z t/\hbar}$$

$$16. = e^{-iZ_2 b t/\hbar} \begin{bmatrix} 1 & 0 & 0 & 0 \\ 0 & 0 & 0 & 0 \\ 0 & 0 & 0 & 0 \\ 0 & 0 & 0 & 0 \end{bmatrix} e^{iZ_2 b t/\hbar}$$

17. + value corresponding
to a π rotation around Z-axis

$$18. \frac{b t}{2\hbar} = \frac{\pi}{2}$$

$$19. t = \frac{2\pi\hbar}{2b} = \frac{\pi\hbar}{b}$$

Calculations For T_1 Noise

1. Redefine σ_+ to target second qubit

$$2. \sigma_{+2} \equiv I \otimes \sigma_+ = \begin{bmatrix} 1 & 0 \\ 0 & 1 \end{bmatrix} \otimes \begin{bmatrix} 0 & 1 \\ 0 & 0 \end{bmatrix}$$

$$3. = \begin{bmatrix} 1 \begin{bmatrix} 0 & 1 \\ 0 & 0 \end{bmatrix} & 0 \begin{bmatrix} 0 & 1 \\ 0 & 0 \end{bmatrix} \\ 0 \begin{bmatrix} 0 & 1 \\ 0 & 0 \end{bmatrix} & 1 \begin{bmatrix} 0 & 1 \\ 0 & 0 \end{bmatrix} \end{bmatrix} = \begin{bmatrix} 0 & 1 & 0 & 0 \\ 0 & 0 & 0 & 0 \\ 0 & 0 & 0 & 1 \\ 0 & 0 & 0 & 0 \end{bmatrix}$$

4. Redefine σ_- to target second qubit

$$5. \sigma_{-2} \equiv I \otimes \sigma_- = \begin{bmatrix} 1 & 0 \\ 0 & 1 \end{bmatrix} \otimes \begin{bmatrix} 0 & 0 \\ 1 & 0 \end{bmatrix}$$

$$6. = \begin{bmatrix} 1 \begin{bmatrix} 0 & 0 \\ 1 & 0 \end{bmatrix} & 0 \begin{bmatrix} 0 & 0 \\ 1 & 0 \end{bmatrix} \\ 0 \begin{bmatrix} 0 & 0 \\ 1 & 0 \end{bmatrix} & 1 \begin{bmatrix} 0 & 0 \\ 1 & 0 \end{bmatrix} \end{bmatrix} = \begin{bmatrix} 0 & 0 & 0 & 0 \\ 1 & 0 & 0 & 0 \\ 0 & 0 & 0 & 0 \\ 0 & 0 & 1 & 0 \end{bmatrix}$$

7. Solve $\sigma_{+1} \rho \sigma_{-1}$

$$8. \sigma_{+2} \rho \sigma_{-2} = \begin{bmatrix} 0 & 1 & 0 & 0 \\ 0 & 0 & 0 & 0 \\ 0 & 0 & 0 & 1 \\ 0 & 0 & 0 & 0 \end{bmatrix} e^{-iHt/\hbar} \begin{bmatrix} 1 & 0 & 0 & 0 \\ 0 & 0 & 0 & 0 \\ 0 & 0 & 0 & 0 \\ 0 & 0 & 0 & 0 \end{bmatrix} e^{iHt/\hbar} \begin{bmatrix} 0 & 0 & 0 & 0 \\ 1 & 0 & 0 & 0 \\ 0 & 0 & 0 & 0 \\ 0 & 0 & 1 & 0 \end{bmatrix}$$

$$9. = e^{-iHt/\hbar} \begin{bmatrix} 0 & 1 & 0 & 0 \\ 0 & 0 & 0 & 0 \\ 0 & 0 & 0 & 1 \\ 0 & 0 & 0 & 0 \end{bmatrix} \begin{bmatrix} 1 & 0 & 0 & 0 \\ 0 & 0 & 0 & 0 \\ 0 & 0 & 0 & 0 \\ 0 & 0 & 0 & 0 \end{bmatrix} \begin{bmatrix} 0 & 0 & 0 & 0 \\ 1 & 0 & 0 & 0 \\ 0 & 0 & 0 & 0 \\ 0 & 0 & 1 & 0 \end{bmatrix} e^{iHt/\hbar}$$

$$10. = e^{-iHt/\hbar} \begin{bmatrix} 0 & 1 & 0 & 0 \\ 0 & 0 & 0 & 0 \\ 0 & 0 & 0 & 1 \\ 0 & 0 & 0 & 0 \end{bmatrix} \begin{bmatrix} 0 & 0 & 0 & 0 \\ 0 & 0 & 0 & 0 \\ 0 & 0 & 0 & 0 \\ 0 & 0 & 0 & 0 \end{bmatrix} e^{iHt/\hbar}$$

$$11. = 0$$

$$12. \text{ solve } \sigma_- \sigma_+ \rho$$

$$13. \sigma_- \sigma_+ \rho =$$

$$e^{-iHt/\hbar} \begin{bmatrix} 0 & 0 & 0 & 0 \\ 1 & 0 & 0 & 0 \\ 0 & 0 & 0 & 0 \\ 0 & 0 & 1 & 0 \end{bmatrix} \begin{bmatrix} 0 & 1 & 0 & 0 \\ 0 & 0 & 0 & 0 \\ 0 & 0 & 0 & 1 \\ 0 & 0 & 0 & 0 \end{bmatrix} \begin{bmatrix} 1 & 0 & 0 & 0 \\ 0 & 0 & 0 & 0 \\ 0 & 0 & 0 & 0 \\ 0 & 0 & 0 & 0 \end{bmatrix} e^{iHt/\hbar}$$

$$14. = e^{-iHt/\hbar} \begin{bmatrix} 0 & 0 & 0 & 0 \\ 1 & 0 & 0 & 0 \\ 0 & 0 & 0 & 0 \\ 0 & 0 & 1 & 0 \end{bmatrix} \begin{bmatrix} 0 & 0 & 0 & 0 \\ 0 & 0 & 0 & 0 \\ 0 & 0 & 0 & 0 \\ 0 & 0 & 0 & 0 \end{bmatrix} e^{iHt/\hbar}$$

$$15. = 0$$

$$16. \rho \sigma_- \sigma_+ =$$

$$e^{-iHt/\hbar} \begin{bmatrix} 1 & 0 & 0 & 0 \\ 0 & 0 & 0 & 0 \\ 0 & 0 & 0 & 0 \\ 0 & 0 & 0 & 0 \end{bmatrix} \begin{bmatrix} 0 & 0 & 0 & 0 \\ 1 & 0 & 0 & 0 \\ 0 & 0 & 0 & 0 \\ 0 & 0 & 1 & 0 \end{bmatrix} \begin{bmatrix} 0 & 1 & 0 & 0 \\ 0 & 0 & 0 & 0 \\ 0 & 0 & 0 & 1 \\ 0 & 0 & 0 & 0 \end{bmatrix} e^{iHt/\hbar}$$

$$17. = e^{-iHt/\hbar} \begin{bmatrix} 1 & 0 & 0 & 0 \\ 0 & 0 & 0 & 0 \\ 0 & 0 & 0 & 0 \\ 0 & 0 & 0 & 0 \end{bmatrix} \begin{bmatrix} 0 & 0 & 0 & 0 \\ 0 & 1 & 0 & 0 \\ 0 & 0 & 0 & 0 \\ 0 & 0 & 0 & 1 \end{bmatrix} e^{iHt/\hbar}$$

$$18. = 0$$

19. Add up terms for T_1 Noise

$$20. \frac{d\rho}{dt} = \gamma_+ \left[0 - \frac{1}{2} (0+0) \right]$$

$$21. = 0$$

Calculations For T_1 Noise

1. Initial State $|0\rangle$

2. $\rho(0) = |0\rangle\langle 0|$

3. $= \begin{bmatrix} 0 \\ 1 \\ 0 \\ 0 \end{bmatrix} \begin{bmatrix} 0 & 1 & 0 & 0 \end{bmatrix}$

4. $= \begin{bmatrix} 0 & 0 & 0 & 0 \\ 0 & 1 & 0 & 0 \\ 0 & 0 & 0 & 0 \\ 0 & 0 & 0 & 0 \end{bmatrix}$

5. Unitary operator $U(t)$ - Generic Form

6. $U(t) = e^{-iHt/\hbar}$

7. Form when Hadamard Gate is applied

8. $\rho(t) = U(t) \rho(0) U^\dagger(t)$

9. $= e^{-iH_{12}t/\hbar} \begin{bmatrix} 0 & 0 & 0 & 0 \\ 0 & 1 & 0 & 0 \\ 0 & 0 & 0 & 0 \\ 0 & 0 & 0 & 0 \end{bmatrix} e^{iH_{12}t/\hbar}$

10. $= e^{-iU_H b t/\hbar} \begin{bmatrix} 0 & 0 & 0 & 0 \\ 0 & 1 & 0 & 0 \\ 0 & 0 & 0 & 0 \\ 0 & 0 & 0 & 0 \end{bmatrix} e^{iU_H b t/\hbar}$

11. solve $\sigma_z \rho \sigma_z$

12. $\sigma_z \rho \sigma_z =$

$$e^{-iHt/\hbar} \begin{bmatrix} 0 & 1 & 0 & 0 \\ 0 & 0 & 0 & 0 \\ 0 & 0 & 0 & 1 \\ 0 & 0 & 0 & 0 \end{bmatrix} \begin{bmatrix} 0 & 0 & 0 & 0 \\ 0 & 1 & 0 & 0 \\ 0 & 0 & 0 & 0 \\ 0 & 0 & 0 & 0 \end{bmatrix} \begin{bmatrix} 0 & 0 & 0 & 0 \\ 0 & 1 & 0 & 0 \\ 0 & 0 & 0 & 0 \\ 0 & 0 & 1 & 0 \end{bmatrix} e^{iHt/\hbar}$$

13. $=$

$$e^{-iHt/\hbar} \begin{bmatrix} 0 & 1 & 0 & 0 \\ 0 & 0 & 0 & 0 \\ 0 & 0 & 0 & 1 \\ 0 & 0 & 0 & 0 \end{bmatrix} \begin{bmatrix} 0 & 0 & 0 & 0 \\ 0 & 1 & 0 & 0 \\ 0 & 0 & 0 & 0 \\ 0 & 0 & 0 & 0 \end{bmatrix} e^{iHt/\hbar}$$

14. $=$

$$e^{-iHt/\hbar} \begin{bmatrix} 1 & 0 & 0 & 0 \\ 0 & 0 & 0 & 0 \\ 0 & 0 & 0 & 0 \\ 0 & 0 & 0 & 0 \end{bmatrix} e^{iHt/\hbar}$$

15. solve $\sigma_z \rho \sigma_z$

16. $\sigma_z \rho \sigma_z =$

$$e^{-iHt/\hbar} \begin{bmatrix} 0 & 0 & 0 & 0 \\ 0 & 1 & 0 & 0 \\ 0 & 0 & 0 & 0 \\ 0 & 0 & 1 & 0 \end{bmatrix} \begin{bmatrix} 0 & 1 & 0 & 0 \\ 0 & 0 & 0 & 0 \\ 0 & 0 & 0 & 1 \\ 0 & 0 & 0 & 0 \end{bmatrix} \begin{bmatrix} 0 & 0 & 0 & 0 \\ 0 & 1 & 0 & 0 \\ 0 & 0 & 0 & 0 \\ 0 & 0 & 0 & 0 \end{bmatrix} e^{iHt/\hbar}$$

17. $=$

$$e^{-iHt/\hbar} \begin{bmatrix} 0 & 0 & 0 & 0 \\ 0 & 1 & 0 & 0 \\ 0 & 0 & 0 & 0 \\ 0 & 0 & 1 & 0 \end{bmatrix} \begin{bmatrix} 0 & 1 & 0 & 0 \\ 0 & 0 & 0 & 0 \\ 0 & 0 & 0 & 0 \\ 0 & 0 & 0 & 0 \end{bmatrix} e^{iHt/\hbar}$$

18. $=$

$$e^{-iHt/\hbar} \begin{bmatrix} 0 & 0 & 0 & 0 \\ 0 & 1 & 0 & 0 \\ 0 & 0 & 0 & 0 \\ 0 & 0 & 0 & 0 \end{bmatrix} e^{iHt/\hbar}$$

19. solve $\rho\sigma_z\rho + 2$

20. $\rho\sigma_z\rho + 2 =$

$$e^{-iHt/\hbar} \begin{bmatrix} 0 & 0 & 0 & 0 \\ 0 & 1 & 0 & 0 \\ 0 & 0 & 0 & 0 \\ 0 & 0 & 0 & 0 \end{bmatrix} \begin{bmatrix} 0 & 0 & 0 & 0 \\ 1 & 0 & 0 & 0 \\ 0 & 0 & 0 & 0 \\ 0 & 0 & 1 & 0 \end{bmatrix} \begin{bmatrix} 0 & 1 & 0 & 0 \\ 0 & 0 & 0 & 0 \\ 0 & 0 & 0 & 1 \\ 0 & 0 & 0 & 0 \end{bmatrix} e^{iHt/\hbar}$$

21. $=$

$$e^{-iHt/\hbar} \begin{bmatrix} 0 & 0 & 0 & 0 \\ 0 & 1 & 0 & 0 \\ 0 & 0 & 0 & 0 \\ 0 & 0 & 0 & 0 \end{bmatrix} \begin{bmatrix} 0 & 0 & 0 & 0 \\ 0 & 1 & 0 & 0 \\ 0 & 0 & 0 & 0 \\ 0 & 0 & 0 & 1 \end{bmatrix} e^{iHt/\hbar}$$

22. $=$

$$e^{-iHt/\hbar} \begin{bmatrix} 0 & 0 & 0 & 0 \\ 0 & 1 & 0 & 0 \\ 0 & 0 & 0 & 0 \\ 0 & 0 & 0 & 0 \end{bmatrix} e^{iHt/\hbar}$$

23. Add terms to find T_1 Noise

24. $\frac{d\rho}{dt} =$

$$\gamma_+ \left[e^{-iHt/\hbar} \left(\begin{bmatrix} 1 & 0 & 0 & 0 \\ 0 & 0 & 0 & 0 \\ 0 & 0 & 0 & 0 \\ 0 & 0 & 0 & 0 \end{bmatrix} - \frac{1}{2} \left(\begin{bmatrix} 0 & 0 & 0 & 0 \\ 0 & 1 & 0 & 0 \\ 0 & 0 & 0 & 0 \\ 0 & 0 & 0 & 0 \end{bmatrix} + \begin{bmatrix} 0 & 0 & 0 & 0 \\ 0 & 1 & 0 & 0 \\ 0 & 0 & 0 & 0 \\ 0 & 0 & 0 & 0 \end{bmatrix} \right) \right) e^{iHt/\hbar} \right]$$

25. $=$

$$\gamma_+ \left[e^{-iHt/\hbar} \left(\begin{bmatrix} 1 & 0 & 0 & 0 \\ 0 & 0 & 0 & 0 \\ 0 & 0 & 0 & 0 \\ 0 & 0 & 0 & 0 \end{bmatrix} - \frac{1}{2} \left(\begin{bmatrix} 0 & 0 & 0 & 0 \\ 0 & 1 & 0 & 0 \\ 0 & 0 & 0 & 0 \\ 0 & 0 & 0 & 0 \end{bmatrix} \right) \right) e^{iHt/\hbar} \right]$$

$$26. = \gamma_+ [e^{-iH+\hbar} \left(\begin{bmatrix} 1 & 0 & 0 & 0 \\ 0 & 0 & 0 & 0 \\ 0 & 0 & 0 & 0 \\ 0 & 0 & 0 & 0 \end{bmatrix} - \begin{bmatrix} 0 & 0 & 0 & 0 \\ 0 & 1 & 0 & 0 \\ 0 & 0 & 0 & 0 \\ 0 & 0 & 0 & 0 \end{bmatrix} \right) e^{iH+\hbar}]$$

$$27. = \gamma_+ [e^{-iH+\hbar} \begin{bmatrix} 1 & 0 & 0 & 0 \\ 0 & -1 & 0 & 0 \\ 0 & 0 & 0 & 0 \\ 0 & 0 & 0 & 0 \end{bmatrix} e^{iH+\hbar}]$$